src/Pact.v
@@ -1,0 +1,152 @@
+Require Export
+  Coq.ZArith.ZArith
+  Ty
+  Exp
+  Sub
+  Sem
+  Eval
+  Norm
+  CEK.
+
+From Equations Require Import Equations.
+Set Equations With UIP.
+
+Generalizable All Variables.
+
+Section Pact.
+
+Import ListNotations.
+
+Open Scope Ty_scope.
+Open Scope Z_scope.
+
+Inductive Pact := PactLang.     (* this is just a type-level tag *)
+
+Inductive PactTy := TyInteger.
+
+Derive NoConfusion for PactTy.
+
+Definition Pact_HostTypes : HostTypes Pact := {|
+  HostTy := PactTy;
+  HostTySem := λ ty,
+    match ty with
+    | TyInteger => Z
+    end
+|}.
+
+Inductive PactExp : Ty (H:=Pact_HostTypes) → Type :=
+  | PInteger : Z → PactExp (TyHost (H:=Pact_HostTypes) TyInteger)
+  | FAdd : PactExp (TyHost (H:=Pact_HostTypes) TyInteger ×
+                    TyHost (H:=Pact_HostTypes) TyInteger
+                      ⟶ TyHost (H:=Pact_HostTypes) TyInteger).
+
+Derive Signature NoConfusion Subterm for PactExp.
+
+Definition Pact_HostExprs : HostExprs Pact := {|
+  has_host_types := Pact_HostTypes;
+  HostExp := PactExp
+|}.
+
+Equations Pact_HostExpSem `(e : HostExp (HostExprs:=Pact_HostExprs) τ) : SemTy τ :=
+  Pact_HostExpSem (PInteger z) := z;
+  Pact_HostExpSem FAdd := λ '(x, y), x + y.
+
+(*
+Definition PactF {dom cod : Ty (H:=@has_host_types _ Pact_HostExprs)}
+           `(e : PactExp (dom ⟶ cod))
+           `(v : Exp Γ dom) (V : ValueP v) : Exp Γ cod :=
+  match e with
+  | FAdd =>
+      match V with
+      | PairP (@HostedP _ ?(@has_host_types _ Pact_HostExprs) _ _ (PInteger x))
+              (HostedP (PInteger y)) => Hosted (PInteger (x + y))
+      | _ => !
+      end
+  | _ => !
+  end.
+*)
+
+Equations PactF {dom cod : Ty (H:=@has_host_types _ Pact_HostExprs)}
+          (e : PactExp (dom ⟶ cod))
+          `(v : Exp Γ dom) (V : ValueP v) : Exp Γ cod :=
+  PactF FAdd (Pair (Hosted (PInteger x)) (Hosted (PInteger y))) _ :=
+    Hosted (H:=Pact_HostExprs) (PInteger (x + y));
+  PactF FAdd _ _ := _.
+Next Obligation. now inv h. Defined.
+Next Obligation. now inv V. Defined.
+Next Obligation. now inv V. Defined.
+Next Obligation. now inv V. Defined.
+Next Obligation. now inv V. Defined.
+Next Obligation. now inv V. Defined.
+Next Obligation. now inv V. Defined.
+Next Obligation. now inv V. Defined.
+Next Obligation. now inv V. Defined.
+Next Obligation. now inv V. Defined.
+Next Obligation. now inv V. Defined.
+
+Program Instance Pact_HostExprsSem : HostExprsSem Pact := {|
+  has_host_exprs := Pact_HostExprs;
+  HostExpSem := @Pact_HostExpSem;
+  CallHost := λ Γ dom cod f, @PactF dom cod f Γ;
+  GetBool := λ _ x, exist _ _ _;
+  GetPair := λ _ _ _ x, exist _ _ _;
+|}.
+Next Obligation. now inv X0. Defined.
+Next Obligation. now inv x. Defined.
+Next Obligation. now inv x. Defined.
+Next Obligation. now inv x. Defined.
+Next Obligation. now inv x. Defined.
+Next Obligation. now inv x. Defined.
+
+Program Instance Pact_HostLang : HostLang Pact := {|
+  has_host_exprs_sem := Pact_HostExprsSem;
+|}.
+Next Obligation.
+  dependent induction f; simp Pact_HostExpSem.
+  dependent elimination v; simp PactF; inversion H.
+  reduce.
+  simp PactF; simpl.
+  inv X; inv X0.
+  dependent elimination x.
+  dependent elimination x0.
+  simp PactF; simpl.
+  now simp Pact_HostExpSem.
+Qed.
+Next Obligation. Admitted.
+Next Obligation. Admitted.
+Next Obligation. Admitted.
+Next Obligation. Admitted.
+Next Obligation. Admitted.
+Next Obligation. Admitted.
+Next Obligation. Admitted.
+Next Obligation. Admitted.
+Next Obligation. Admitted.
+Next Obligation. Admitted.
+Next Obligation. Admitted.
+Next Obligation. Admitted.
+
+Example exp_constant :
+  run 10 (Hosted (PInteger 123)) = MkΣ (Hosted (PInteger 123)) Empty MT.
+Proof. reflexivity. Qed.
+
+Example exp_pair :
+  run 20 (Pair (Hosted (PInteger 123))
+               (Hosted (PInteger 456))) =
+    MkΣ (Pair (Hosted (PInteger 123)) (Hosted (PInteger 456))) Empty MT.
+Proof. reflexivity. Qed.
+
+Example exp_lam τ :
+  run 10 (LAM (cod:=τ) (VAR ZV)) = MkΣ (LAM (VAR ZV)) Empty MT.
+Proof. reflexivity. Qed.
+
+Example exp_app :
+  run 10 (APP (LAM (VAR ZV)) (Hosted (PInteger 123))) =
+    MkΣ (Hosted (PInteger 123)) Empty MT.
+Proof. reflexivity. Qed.
+
+Example exp_call_FAdd :
+  run 10 (APP (Hosted FAdd) (Pair (Hosted (PInteger 123)) (Hosted (PInteger 456)))) =
+    MkΣ (Hosted (PInteger 579)) Empty MT.
+Proof. reflexivity. Qed.
+
+End Pact.
